more proofs!

twophase/Twophase/Proofs.lean
@@ -12,6 +12,7 @@ Authors: Igor Konnov, 2025
 
 import Twophase.Propositional
 import Mathlib.Data.Finset.Basic
+import Std.Data.HashMap.Lemmas
 
 -- The abstract type of resource managers.
 variable { RM : Type } [DecidableEq RM] [Hashable RM]
@@ -41,11 +42,11 @@ def lemma4 (s: ProtocolState RM) : Prop :=
 
 def lemma5 (s: ProtocolState RM) : Prop :=
   Message.Abort ∈ s.msgs →
-    s.tmState = TMState.Aborted
+    (s.tmState = TMState.Aborted
       ∨ ∃ rm: RM,
           s.rmState[rm]? = some RMState.Aborted
         ∧ rm ∉ s.tmPrepared
-        ∧ Message.Prepared rm ∉ s.msgs
+        ∧ Message.Prepared rm ∉ s.msgs)
 
 def lemma6 (s: ProtocolState RM) : Prop :=
   Message.Commit ∈ s.msgs →
@@ -88,8 +89,121 @@ lemma invariant_is_inductive_tm_abort_lemma1 (s: ProtocolState RM) (s': Protocol
         exact h_lemma1
       -- s.tmState = TMState.Committed contradicts s.tmState = TMState.Init
       have h_tm_init: s.tmState = TMState.Init := by simp [h_tm_abort]
+      -- prove the contradiction
       simp [h_tm_init] at h_tm_committed
     simp [h_no_committed]
+
+-- Effort: 20m
+lemma invariant_is_inductive_tm_receive_prepared_lemma1 (s: ProtocolState RM) (s': ProtocolState RM)
+  (rm: RM) (h_inv: invariant s) (h_tm_rcv_prepared: tm_rcv_prepared s s' rm): lemma1 s' := by
+    unfold lemma1
+    unfold tm_rcv_prepared at h_tm_rcv_prepared
+    have h_tm_state_init: s.tmState = TMState.Init := by simp [h_tm_rcv_prepared]
+    have h_tm_state_not_committed: s'.tmState ≠ TMState.Committed := by
+      have h_unchanged_tm_state: s'.tmState = s.tmState := by simp [h_tm_rcv_prepared]
+      simp [h_unchanged_tm_state, h_tm_state_init]
+    simp [h_tm_state_not_committed]
+    intro rm
+    by_contra h_some_committed -- assume the opposite
+    have h_unchanged_rm_state: s'.rmState = s.rmState := by simp [h_tm_rcv_prepared]
+    simp [h_unchanged_rm_state] at h_some_committed
+    rcases h_inv with ⟨h_lemma1_s, _, _, _, _, _⟩
+    unfold lemma1 at h_lemma1_s
+    have h_ex_committed: ∃ rm: RM, s.rmState[rm]? = some RMState.Committed := by exists rm
+    simp [h_ex_committed] at h_lemma1_s
+    simp [h_tm_state_init] at h_lemma1_s
+
+-- Effort: 1h
+lemma invariant_is_inductive_rm_prepare_lemma1 (s: ProtocolState RM) (s': ProtocolState RM)
+  (rm: RM) (h_inv: invariant s) (h_rm_prepare: rm_prepare s s' rm): lemma1 s' := by
+    unfold lemma1
+    unfold rm_prepare at h_rm_prepare
+    rcases h_inv with ⟨h_lemma1_s, _, _, _, _, _⟩
+    unfold lemma1 at h_lemma1_s
+    by_cases h_some_committed: ∃ rm: RM, s.rmState[rm]? = some RMState.Committed
+    case neg =>
+      simp [*] at h_some_committed
+      have h_all_not_committed: ∀ (x : RM), s'.rmState[x]? ≠ some RMState.Committed := by
+        intro rm₂
+        have h_rm_state: s'.rmState = s.rmState.insert rm RMState.Prepared := by
+          simp [h_rm_prepare]
+        simp [h_rm_state]
+        simp [Std.HashMap.getElem?_insert]
+        specialize h_some_committed rm₂
+        split
+        . simp
+        . simp [h_some_committed]
+      simp [h_all_not_committed]
+
+    case pos =>
+      rcases h_some_committed with ⟨rm₂, h_rm2_committed⟩
+      have h_rm2_neq_rm : rm₂ ≠ rm := by
+        by_contra h_contra -- assume the opposite
+        have h_rm_state_working : s.rmState.get? rm = some RMState.Working := by
+          rcases h_rm_prepare with ⟨h_rm_state, _⟩
+          exact h_rm_state
+        simp [h_contra] at h_rm2_committed
+        simp [h_rm2_committed] at h_rm_state_working
+      have h_rm_state_committed: s'.rmState.get? rm₂ = some RMState.Committed := by
+        have h_rm_state: s'.rmState = s.rmState.insert rm RMState.Prepared :=
+          by simp [h_rm_prepare]
+        simp [h_rm_state]
+        simp [Std.HashMap.getElem?_insert]
+        have : rm ≠ rm₂ := by
+          intro h_contra -- assume the opposite
+          simp [h_contra] at h_rm2_neq_rm
+        simp [this]
+        exact h_rm2_committed
+
+      have h_some_committed_pre: ∃ rm: RM, s.rmState[rm]? = some RMState.Committed := by use rm₂
+      have h_some_committed_post: ∃ rm: RM, s'.rmState[rm]? = some RMState.Committed := by
+        use rm₂; exact h_rm_state_committed
+      simp [h_some_committed_pre] at h_lemma1_s
+      have h_unchanged_tm_state: s'.tmState = s.tmState := by simp [h_rm_prepare]
+      simp [h_some_committed_post, h_unchanged_tm_state, h_lemma1_s]
+
+-- Effort: 30m
+lemma invariant_is_inductive_rm_abort_lemma1 (s: ProtocolState RM) (s': ProtocolState RM)
+  (rm: RM) (h_inv: invariant s) (h_rm_abort: rm_choose_to_abort s s' rm): lemma1 s' := by
+    unfold lemma1
+    unfold rm_choose_to_abort at h_rm_abort
+    rcases h_inv with ⟨h_lemma1_s, h_lemma2_s, _, _, _, _⟩
+    have h_unchanged_tm_state: s'.tmState = s.tmState := by simp [h_rm_abort]
+    have h_tm_not_committed: s'.tmState ≠ TMState.Committed := by
+      by_contra h_contra -- assume the opposite
+      simp [h_unchanged_tm_state] at h_contra
+      unfold lemma2 at h_lemma2_s
+      simp [h_contra] at h_lemma2_s
+      rcases h_lemma2_s with ⟨_, _, h_no_working⟩
+      specialize h_no_working rm
+      have h_rm_not_working: s.rmState[rm]? ≠ some RMState.Working := by simp [h_no_working]
+      simp [h_rm_not_working] at h_rm_abort
+    simp [h_tm_not_committed]
+    intro rm₂
+    by_cases h_rm2_eq_rm: rm = rm₂
+    case pos =>
+      rw [h_rm2_eq_rm] at h_rm_abort
+      have h_rm2_aborted: s'.rmState[rm]? = some RMState.Aborted := by
+        rcases h_rm_abort with ⟨_, h_rm2_aborted, _⟩
+        simp [h_rm2_aborted]
+        simp [Std.HashMap.getElem?_insert, h_rm2_eq_rm]
+      simp [h_rm2_eq_rm] at h_rm2_aborted
+      simp [h_rm2_aborted]
+
+    case neg =>
+      have h_rm2_state_unchanged: s'.rmState[rm₂]? = s.rmState[rm₂]? := by
+        rcases h_rm_abort with ⟨_, h_rm_state_insert, _, _⟩
+        simp [h_rm_state_insert]
+        simp [Std.HashMap.getElem?_insert, h_rm2_eq_rm]
+      simp [h_rm2_state_unchanged]
+      have h_rm2_not_committed: s.rmState[rm₂]? ≠ RMState.Committed := by
+        by_contra h_contra -- assume the opposite
+        unfold lemma1 at h_lemma1_s
+        have h_ex_committed: ∃ rm: RM, s.rmState[rm]? = some RMState.Committed := by use rm₂
+        simp [h_ex_committed] at h_lemma1_s
+        rw [← h_unchanged_tm_state] at h_lemma1_s
+        simp [h_tm_not_committed] at h_lemma1_s
+      exact h_rm2_not_committed
 
 -- Effort: 3.5h
 lemma invariant_is_inductive_tm_commit_lemma2 (s: ProtocolState RM) (s': ProtocolState RM)
@@ -140,6 +254,76 @@ lemma invariant_is_inductive_tm_commit_lemma2 (s: ProtocolState RM) (s': Protoco
           apply h_prepared_notin_msgs at this -- contradiction
           exact this
 
+-- Effort: 2m
+lemma invariant_is_inductive_tm_abort_lemma2 (s: ProtocolState RM) (s': ProtocolState RM)
+  (h_tm_abort: tm_abort s s'): lemma2 s' := by
+    unfold lemma2
+    unfold tm_abort at h_tm_abort
+    have h_tm_state_aborted : s'.tmState = TMState.Aborted := by simp [h_tm_abort]
+    simp [h_tm_abort]
+
+-- Effort: 2m
+lemma invariant_is_inductive_tm_receive_prepared_lemma2 (s: ProtocolState RM) (s': ProtocolState RM)
+  (rm: RM) (h_tm_rcv_prepared: tm_rcv_prepared s s' rm): lemma2 s' := by
+    unfold lemma2
+    unfold tm_rcv_prepared at h_tm_rcv_prepared
+    have h_tm_state_init: s.tmState = TMState.Init := by simp [h_tm_rcv_prepared]
+    have h_tm_state_not_committed: s'.tmState ≠ TMState.Committed := by
+      have h_unchanged_tm_state: s'.tmState = s.tmState := by simp [h_tm_rcv_prepared]
+      simp [h_unchanged_tm_state, h_tm_state_init]
+    simp [h_tm_state_not_committed]
+
+-- Effort: 30m
+lemma invariant_is_inductive_rm_prepare_lemma2 (s: ProtocolState RM) (s': ProtocolState RM)
+  (rm: RM) (h_inv: invariant s) (h_rm_prepare: rm_prepare s s' rm): lemma2 s' := by
+    unfold lemma2
+    unfold rm_prepare at h_rm_prepare
+    have h_unchanged_tm_state: s'.tmState = s.tmState := by simp [h_rm_prepare]
+    have h_unchanged_tm_prepared: s'.tmPrepared = s.tmPrepared := by simp [h_rm_prepare]
+    have h_unchanged_all: s'.all = s.all := by simp [h_rm_prepare]
+    simp [h_unchanged_tm_state, h_unchanged_tm_prepared, h_rm_prepare]
+    rcases h_inv with ⟨_, h_lemma2_s, _, _, _, _⟩
+    unfold lemma2 at h_lemma2_s
+    by_cases h_committed: s.tmState = TMState.Committed
+    case neg =>
+      simp [h_committed]
+
+    case pos =>
+      simp [h_committed] at h_lemma2_s
+      rcases h_lemma2_s with ⟨h_tm_prepared_eq_all, h_commit_msg, h_no_working⟩
+      simp [h_committed, h_tm_prepared_eq_all, h_commit_msg]
+      intro rm₂ -- ∀ rm: RM
+      by_cases h_rm2_eq_rm: rm = rm₂
+      case pos => -- rm = rm₂
+        simp [h_rm2_eq_rm]
+
+      case neg => -- rm ≠ rm₂
+        simp [Std.HashMap.getElem?_insert]
+        have : rm ≠ rm₂ := by intro h_contra; simp [h_contra] at h_rm2_eq_rm
+        simp [h_rm2_eq_rm]
+        specialize h_no_working rm₂
+        exact h_no_working
+
+-- Effort: 10m
+lemma invariant_is_inductive_rm_abort_lemma2 (s: ProtocolState RM) (s': ProtocolState RM)
+  (rm: RM) (h_inv: invariant s) (h_rm_abort: rm_choose_to_abort s s' rm): lemma2 s' := by
+    unfold lemma2
+    unfold rm_choose_to_abort at h_rm_abort
+    have h_unchanged_tm_state: s'.tmState = s.tmState := by simp [h_rm_abort]
+    simp [h_unchanged_tm_state]
+    have h_tm_not_committed: s.tmState ≠ TMState.Committed := by
+      by_contra h_tm_committed -- assume the opposite
+      rcases h_inv with ⟨_, h_lemma2_s, _, _, _, _⟩
+      unfold lemma2 at h_lemma2_s
+      simp [h_tm_committed] at h_lemma2_s
+      rcases h_lemma2_s with ⟨_, _, h_no_working⟩
+      specialize h_no_working rm
+      have h_rm_working: s.rmState[rm]? = some RMState.Working := by
+        rcases h_rm_abort with ⟨h_rm_is_working, _⟩
+        exact h_rm_is_working
+      simp [h_rm_working] at h_no_working
+    simp [h_tm_not_committed]
+
 -- Effort: 5m
 lemma invariant_is_inductive_tm_commit_lemma3 (s: ProtocolState RM) (s': ProtocolState RM)
   (h_tm_commit: tm_commit s s'):
@@ -148,6 +332,41 @@ lemma invariant_is_inductive_tm_commit_lemma3 (s: ProtocolState RM) (s': Protoco
     unfold tm_commit at h_tm_commit
     have : s'.tmState = TMState.Committed := by simp [h_tm_commit]
     simp [this]
+
+-- Effort: 3m
+lemma invariant_is_inductive_tm_abort_lemma3 (s: ProtocolState RM) (s': ProtocolState RM)
+  (h_tm_abort: tm_abort s s'): lemma3 s' := by
+    unfold lemma3
+    unfold tm_abort at h_tm_abort
+    have : s'.tmState = TMState.Aborted := by simp [h_tm_abort]
+    simp [this]
+    have : Message.Abort ∈ s'.msgs := by simp [h_tm_abort]
+    assumption
+
+-- Effort: 2m
+lemma invariant_is_inductive_tm_receive_prepared_lemma3 (s: ProtocolState RM) (s': ProtocolState RM)
+  (rm: RM) (h_tm_rcv_prepared: tm_rcv_prepared s s' rm): lemma3 s' := by
+    unfold lemma3
+    unfold tm_rcv_prepared at h_tm_rcv_prepared
+    have h_tm_state_init: s.tmState = TMState.Init := by simp [h_tm_rcv_prepared]
+    have h_tm_state_not_committed: s'.tmState ≠ TMState.Aborted := by
+      have h_unchanged_tm_state: s'.tmState = s.tmState := by simp [h_tm_rcv_prepared]
+      simp [h_unchanged_tm_state, h_tm_state_init]
+    simp [h_tm_state_not_committed]
+
+-- Effort: 5m
+lemma invariant_is_inductive_rm_prepare_lemma3 (s: ProtocolState RM) (s': ProtocolState RM)
+  (rm: RM) (h_inv: invariant s) (h_rm_prepare: rm_prepare s s' rm): lemma3 s' := by
+    unfold lemma3
+    unfold rm_prepare at h_rm_prepare
+    have h_unchanged_tm_state: s'.tmState = s.tmState := by simp [h_rm_prepare]
+    have h_abort: Message.Abort ∈ s'.msgs ↔ Message.Abort ∈ s.msgs := by
+      have : s'.msgs = s.msgs ∪ {Message.Prepared rm} := by simp [h_rm_prepare]
+      simp [this]
+    simp [h_unchanged_tm_state, h_abort]
+    rcases h_inv with ⟨_, _, h_lemma3_s, _, _, _⟩
+    unfold lemma3 at h_lemma3_s
+    exact h_lemma3_s
 
 -- Effort: 45m
 lemma invariant_is_inductive_tm_commit_lemma4 (s: ProtocolState RM) (s': ProtocolState RM)
@@ -164,6 +383,113 @@ lemma invariant_is_inductive_tm_commit_lemma4 (s: ProtocolState RM) (s': Protoco
     specialize h_lemma4_s rm
     simp [h_unchanged_rm_state, h_msgs', h_unchanged_tm_prepared]
     exact h_lemma4_s
+
+-- Effort: 15m
+lemma invariant_is_inductive_tm_abort_lemma4 (s: ProtocolState RM) (s': ProtocolState RM)
+  (h_inv: invariant s) (h_tm_abort: tm_abort s s'): lemma4 s' := by
+    unfold lemma4
+    unfold tm_abort at h_tm_abort
+    have h_unchanged_rm_state : s'.rmState = s.rmState := by simp [h_tm_abort]
+    have h_unchanged_tm_prepared: s'.tmPrepared = s.tmPrepared := by simp [h_tm_abort]
+    have h_msgs': s'.msgs = s.msgs ∪ {Message.Abort} := by simp [h_tm_abort]
+    simp [h_unchanged_rm_state, h_unchanged_tm_prepared, h_msgs']
+    unfold invariant at h_inv
+    rcases h_inv with ⟨_, _, _, h_lemma4_s, _, _⟩
+    unfold lemma4 at h_lemma4_s
+    intro rm -- ∀ rm: RM
+    specialize h_lemma4_s rm
+    simp [*] at h_lemma4_s
+    rcases h_lemma4_s with ⟨h_when_tm_prepared, h_no_prepared_in_msgs, h_not_working, _⟩
+    apply And.intro
+    . exact h_when_tm_prepared
+    . apply And.intro
+      . exact h_no_prepared_in_msgs
+      . exact h_not_working
+
+-- Effort: 1h
+lemma invariant_is_inductive_tm_receive_prepared_lemma4 (s: ProtocolState RM) (s': ProtocolState RM)
+  (rm: RM) (h_inv: invariant s) (h_tm_rcv_prepared: tm_rcv_prepared s s' rm): lemma4 s' := by
+    unfold lemma4
+    unfold tm_rcv_prepared at h_tm_rcv_prepared
+    unfold invariant at h_inv
+    rcases h_inv with ⟨_, _, _, h_lemma4_s, _, _⟩
+    unfold lemma4 at h_lemma4_s
+    intro rm' -- ∀ rm: RM
+    by_cases equal: rm' = rm
+    . simp [equal, h_tm_rcv_prepared]
+      specialize h_lemma4_s rm
+      rcases h_lemma4_s with ⟨_, h_rm_is_working, _, h_rm_is_aborted⟩
+      apply And.intro
+      . by_contra h_contra -- assume the opposite
+        simp [h_contra] at h_rm_is_working
+        simp [h_rm_is_working] at h_tm_rcv_prepared
+      . have h_prepared_in_msgs: Message.Prepared rm ∈ s.msgs := by simp [h_tm_rcv_prepared]
+        simp [h_prepared_in_msgs] at h_rm_is_aborted
+        exact h_rm_is_aborted
+    . apply And.intro
+      . intro h_rm_prime_in_prepared
+        have h: s'.tmPrepared = s.tmPrepared ∪ {rm} := by simp [h_tm_rcv_prepared]
+        simp [h, equal] at h_rm_prime_in_prepared
+        have h_unchanged_msgs: s'.msgs = s.msgs := by simp [h_tm_rcv_prepared]
+        have h_unchanged_rm_state: s'.rmState = s.rmState := by simp [h_tm_rcv_prepared]
+        simp [h_unchanged_msgs, h_unchanged_rm_state]
+        specialize h_lemma4_s rm'
+        rcases h_lemma4_s with ⟨h_when_tm_prepared, _, _, _⟩
+        simp [h_rm_prime_in_prepared] at h_when_tm_prepared
+        exact h_when_tm_prepared
+      . have h_unchanged_msgs: s'.msgs = s.msgs := by simp [h_tm_rcv_prepared]
+        have h_unchanged_rm_state: s'.rmState = s.rmState := by simp [h_tm_rcv_prepared]
+        simp [h_unchanged_msgs, h_unchanged_rm_state, equal]
+        specialize h_lemma4_s rm'
+        rcases h_lemma4_s with ⟨_, h_rm_is_working, h_prepared_in_msgs, h_rm_is_aborted⟩
+        apply And.intro
+        . exact h_rm_is_working
+        . apply And.intro
+          . exact h_prepared_in_msgs
+          . exact h_rm_is_aborted
+
+-- Effort: 1h
+lemma invariant_is_inductive_rm_prepare_lemma4 (s: ProtocolState RM) (s': ProtocolState RM)
+  (rm: RM) (h_inv: invariant s) (h_rm_prepare: rm_prepare s s' rm): lemma4 s' := by
+    unfold lemma4
+    unfold rm_prepare at h_rm_prepare
+    intro rm' -- ∀ rm: RM
+    by_cases h_eq: rm = rm'
+    case pos =>
+      rw [← h_eq]
+      have h_rm_prepared: s'.rmState[rm]? = some RMState.Prepared := by simp [h_rm_prepare]
+      have h_rm_not_working: s'.rmState[rm]? ≠ some RMState.Working := by
+        by_contra h_contra -- assume the opposite
+        rw [h_contra] at h_rm_prepared
+        injection h_rm_prepared with h_val_eq
+        injection h_val_eq
+      have h_rm_not_aborted: s'.rmState[rm]? ≠ some RMState.Aborted := by
+        by_contra h_contra -- assume the opposite
+        rw [h_contra] at h_rm_prepared
+        injection h_rm_prepared with h_val_eq
+        injection h_val_eq
+      have h_prepared_in_msgs: Message.Prepared rm ∈ s'.msgs := by simp [h_rm_prepare]
+      simp [h_rm_not_working, h_rm_not_aborted, h_prepared_in_msgs]
+
+    case neg =>
+      -- replace s' with s
+      have h_unchanged_rm_state: s'.rmState[rm']? = s.rmState[rm']? := by
+        rcases h_rm_prepare with ⟨_, h_update_rm_state, _⟩
+        simp [h_update_rm_state, Std.HashMap.getElem?_insert, h_eq]
+      have h_tm_prepared: s'.tmPrepared = s.tmPrepared := by simp [h_rm_prepare]
+      have h_prepared_in_msgs: Message.Prepared rm' ∈ s'.msgs ↔ Message.Prepared rm' ∈ s.msgs := by
+        have h_neq: ¬rm' = rm := by
+          intro h_contra -- assume the opposite
+          simp [h_contra] at h_eq
+        simp [h_rm_prepare, h_neq]
+      have h_abort_in_msgs: Message.Abort ∈ s'.msgs ↔ Message.Abort ∈ s.msgs := by
+        simp [h_rm_prepare]
+      simp [h_unchanged_rm_state, h_tm_prepared, h_prepared_in_msgs, h_abort_in_msgs]
+      -- now we can apply the invariant
+      rcases h_inv with ⟨_, _, _, h_lemma4_s, _, _⟩
+      unfold lemma4 at h_lemma4_s
+      specialize h_lemma4_s rm'
+      exact h_lemma4_s
 
 -- Effort: 25m
 lemma invariant_is_inductive_tm_commit_lemma5 (s: ProtocolState RM) (s': ProtocolState RM)
@@ -196,6 +522,95 @@ lemma invariant_is_inductive_tm_commit_lemma5 (s: ProtocolState RM) (s': Protoco
         exact h_rm2_in_prepared
     simp [this]
 
+-- Effort: 3m
+lemma invariant_is_inductive_tm_abort_lemma5 (s: ProtocolState RM) (s': ProtocolState RM)
+  (h_tm_abort: tm_abort s s'): lemma5 s' := by
+    unfold lemma5
+    unfold tm_abort at h_tm_abort
+    have h_tm_state_aborted : s'.tmState = TMState.Aborted := by simp [h_tm_abort]
+    simp [h_tm_state_aborted]
+
+-- Effort: 1h
+lemma invariant_is_inductive_tm_receive_prepared_lemma5 (s: ProtocolState RM) (s': ProtocolState RM)
+  (rm: RM) (h_inv: invariant s) (h_tm_rcv_prepared: tm_rcv_prepared s s' rm): lemma5 s' := by
+    unfold lemma5
+    unfold tm_rcv_prepared at h_tm_rcv_prepared
+    unfold invariant at h_inv
+    have h_unchanged_msgs: s'.msgs = s.msgs := by simp [h_tm_rcv_prepared]
+    have h_unchanged_tm_state: s'.tmState = s.tmState := by simp [h_tm_rcv_prepared]
+    have h_rm_state: s'.rmState = s.rmState := by simp [h_tm_rcv_prepared]
+    have h_tm_state_init: s.tmState = TMState.Init := by simp [h_tm_rcv_prepared]
+    simp [h_unchanged_msgs, h_unchanged_tm_state, h_rm_state]
+    rcases h_inv with ⟨_, _, _, _, h_lemma5_s, _⟩
+    unfold lemma5 at h_lemma5_s
+    simp [h_tm_state_init] at h_lemma5_s; simp [h_tm_state_init]
+    by_cases h_abort: Message.Abort ∈ s.msgs
+    case neg =>
+      simp [h_abort]
+
+    case pos =>
+      simp [h_abort]; simp [h_abort] at h_lemma5_s
+      rcases h_lemma5_s with ⟨rm₂, ⟨h_rm2_aborted, h_rm2_not_prepared, h_rm2_notin_msgs⟩⟩
+      have h_rm_neq_rm: rm₂ ≠ rm := by
+        by_contra h_contra -- assume the opposite
+        have h_rm_prepared: Message.Prepared rm ∈ s.msgs := by simp [h_tm_rcv_prepared]
+        rw [h_contra] at h_rm2_notin_msgs
+        simp [h_rm_prepared] at h_rm2_notin_msgs
+      have h_rm2_not_prepared: rm₂ ∉ s'.tmPrepared := by
+        have h_tm_prepared: s'.tmPrepared = s.tmPrepared ∪ {rm}:= by simp [h_tm_rcv_prepared]
+        by_contra h_contra -- assume the opposite
+        simp [h_tm_prepared, h_rm_neq_rm] at h_contra
+        simp [h_contra] at h_rm2_not_prepared
+      exists rm₂
+
+-- Effort: 1h
+lemma invariant_is_inductive_rm_prepare_lemma5 (s: ProtocolState RM) (s': ProtocolState RM)
+  (rm: RM) (h_inv: invariant s) (h_rm_prepare: rm_prepare s s' rm): lemma5 s' := by
+    unfold lemma5
+    unfold rm_prepare at h_rm_prepare
+    have h_abort_in_msgs: Message.Abort ∈ s'.msgs ↔ Message.Abort ∈ s.msgs := by
+      simp [h_rm_prepare]
+    have h_unchanged_tm_state: s'.tmState = s.tmState := by simp [h_rm_prepare]
+    simp [h_abort_in_msgs, h_unchanged_tm_state]
+    rcases h_inv with ⟨_, _, _, _, h_lemma5_s, _⟩
+    unfold lemma5 at h_lemma5_s
+    by_cases h_abort: Message.Abort ∈ s.msgs
+    case neg =>
+      simp [h_abort]
+
+    case pos =>
+      simp [h_abort] at h_lemma5_s; simp [h_abort]
+      by_cases h_tm_aborted: s.tmState = TMState.Aborted
+      case pos =>
+        simp [h_tm_aborted]
+
+      case neg =>
+        simp [h_tm_aborted] at h_lemma5_s
+        simp [h_tm_aborted]
+        rcases h_lemma5_s with ⟨rm₂, ⟨h_rm2_aborted, h_rm2_not_prepared, h_rm2_notin_msgs⟩⟩
+        exists rm₂
+        have h_rm_neq_rm2: rm ≠ rm₂ := by
+          by_contra h_contra -- assume the opposite
+          rw [← h_contra] at h_rm2_aborted
+          rcases h_rm_prepare with ⟨h_rm_working, _⟩
+          simp at h_rm_working
+          rw [h_rm2_aborted] at h_rm_working
+          injection h_rm_working with h_val_eq
+          injection h_val_eq
+        have h_unchanged_rm2_state: s'.rmState[rm₂]? = s.rmState[rm₂]? := by
+          rcases h_rm_prepare with ⟨_, h_update_rm_state, _⟩
+          simp [h_update_rm_state, Std.HashMap.getElem?_insert]
+          simp [h_rm_neq_rm2]
+        simp [h_unchanged_rm2_state, h_rm2_aborted]
+        have h_unchanged_tm_prepared: s'.tmPrepared = s.tmPrepared := by simp [h_rm_prepare]
+        simp [h_unchanged_tm_prepared, h_rm2_not_prepared]
+        have h_prepared_in_msgs: Message.Prepared rm₂ ∉ s'.msgs ↔ Message.Prepared rm₂ ∉ s.msgs := by
+          simp [h_rm_prepare, h_rm2_notin_msgs]
+          by_contra h_rm2_eq_rm -- assume the opposite
+          rw [h_rm2_eq_rm] at h_rm_neq_rm2
+          simp at h_rm_neq_rm2
+        simp [h_prepared_in_msgs, h_rm2_notin_msgs]
+
 -- Effort: 5m
 lemma invariant_is_inductive_tm_commit_lemma6
   (s: ProtocolState RM) (s': ProtocolState RM) (h_tm_commit: tm_commit s s'): lemma6 s' := by
@@ -212,6 +627,104 @@ lemma invariant_is_inductive_tm_commit_lemma6
     simp [this]
     have : s'.tmState = TMState.Committed := by simp [h_tm_commit]
     simp [this]
+
+-- Effort: 30m
+lemma invariant_is_inductive_tm_abort_lemma6 (s: ProtocolState RM) (s': ProtocolState RM)
+  (h_inv: invariant s) (h_tm_abort: tm_abort s s'): lemma6 s' := by
+    unfold lemma6
+    unfold tm_abort at h_tm_abort
+    have h_msgs': s'.msgs = s.msgs ∪ {Message.Abort} := by simp [h_tm_abort]
+    simp [h_msgs']
+    have h_tm_state_aborted: s'.tmState = TMState.Aborted := by simp [h_tm_abort]
+    have h_tm_state_init: s.tmState = TMState.Init := by simp [h_tm_abort]
+    simp [h_tm_state_aborted]
+    have h_unchanged_rm_state: s'.rmState = s.rmState := by simp [h_tm_abort]
+    simp [h_unchanged_rm_state]
+    unfold invariant at h_inv
+    rcases h_inv with ⟨h_lemma1_s, _, _, _, _, h_lemma6_s⟩
+    unfold lemma1 at h_lemma1_s
+    have h_no_commit_msg : Message.Commit ∉ s.msgs := by
+      by_contra h_contra -- assume the opposite
+      unfold lemma6 at h_lemma6_s
+      apply h_lemma6_s at h_contra
+      simp [h_tm_state_init] at h_contra
+      have h_no_rm_committed: (∃ rm: RM, s.rmState[rm]? = some RMState.Committed) → False := by
+        intro h_committed
+        simp [h_tm_state_init] at h_lemma1_s
+        rcases h_committed with ⟨rm, h_committed⟩
+        specialize h_lemma1_s rm
+        simp [h_lemma1_s] at h_committed
+      simp [*] at h_no_rm_committed
+    simp [h_no_commit_msg]
+
+-- Effort: 7m
+lemma invariant_is_inductive_tm_receive_prepared_lemma6 (s: ProtocolState RM) (s': ProtocolState RM)
+  (rm: RM) (h_all: ∀ rm: RM, rm ∈ s.all) (h_inv: invariant s) (h_tm_rcv_prepared: tm_rcv_prepared s s' rm): lemma6 s' := by
+    unfold lemma6
+    unfold tm_rcv_prepared at h_tm_rcv_prepared
+    unfold invariant at h_inv
+    have h_unchanged_tm_state: s'.tmState = s.tmState := by simp [h_tm_rcv_prepared]
+    have h_tm_state_init: s.tmState = TMState.Init := by simp [h_tm_rcv_prepared]
+    have h_unchanged_rm_state: s'.rmState = s.rmState := by simp [h_tm_rcv_prepared]
+    have h_unchanged_msgs: s'.msgs = s.msgs := by simp [h_tm_rcv_prepared]
+    simp [h_unchanged_tm_state, h_tm_state_init, h_unchanged_rm_state, h_unchanged_msgs]
+    rcases h_inv with ⟨_, _, _, _, _, h_lemma6_s⟩
+    unfold lemma6 at h_lemma6_s
+    by_cases h_commit: Message.Commit ∈ s.msgs
+    case neg =>
+      simp [h_commit]
+
+    case pos =>
+      simp [h_commit]
+      simp [h_commit] at h_lemma6_s
+      simp [h_tm_state_init] at h_lemma6_s
+      rcases h_lemma6_s with ⟨h_tm_prepared_eq_all, h_rm_state_committed⟩
+      simp [h_rm_state_committed]
+      have h_unchanged_all: s'.all = s.all := by simp [h_tm_rcv_prepared]
+      simp [h_unchanged_all]
+      have h_tm_prepared: s'.tmPrepared = s.tmPrepared ∪ {rm} := by simp [h_tm_rcv_prepared]
+      rw [h_tm_prepared, h_tm_prepared_eq_all]
+      simp [h_all]
+
+-- Effort: 20m
+lemma invariant_is_inductive_rm_prepare_lemma6 (s: ProtocolState RM) (s': ProtocolState RM)
+  (rm: RM) (h_inv: invariant s) (h_rm_prepare: rm_prepare s s' rm): lemma6 s' := by
+    unfold lemma6
+    unfold rm_prepare at h_rm_prepare
+    have h_commit_in_msgs: Message.Commit ∈ s'.msgs ↔ Message.Commit ∈ s.msgs := by
+      simp [h_rm_prepare]
+    have h_unchanged_tm_state: s'.tmState = s.tmState := by simp [h_rm_prepare]
+    have h_unchanged_tm_prepared: s'.tmPrepared = s.tmPrepared := by simp [h_rm_prepare]
+    have h_unchanged_all: s'.all = s.all := by simp [h_rm_prepare]
+    simp [h_commit_in_msgs, h_unchanged_tm_state, h_unchanged_tm_prepared, h_unchanged_all]
+    by_cases h_commit: Message.Commit ∈ s.msgs
+    case neg =>
+      simp [h_commit]
+
+    case pos =>
+      simp [h_commit]
+      rcases h_inv with ⟨_, _, _, _, _, h_lemma6_s⟩
+      unfold lemma6 at h_lemma6_s
+      simp [h_commit] at h_lemma6_s
+      rcases h_lemma6_s with ⟨h_tm_prepared_eq_all, h_tm_committed_or_rm_committed⟩
+      simp [h_tm_prepared_eq_all]
+      cases h_tm_committed_or_rm_committed
+      case inl h_tm_state_committed =>
+        simp [h_tm_state_committed]
+
+      case inr h_rm_state_committed =>
+        rcases h_rm_state_committed with ⟨rm₂, h_rm2_committed⟩
+        have h_rm2_neq_rm:  rm ≠ rm₂ := by
+          by_contra h_contra -- assume the opposite
+          rw [← h_contra] at h_rm2_committed
+          simp [h_rm2_committed] at h_rm_prepare
+        have h_rm2_committed: s'.rmState[rm₂]? = RMState.Committed := by
+          rcases h_rm_prepare with ⟨_, h_update_rm_state, _⟩
+          simp [h_update_rm_state, Std.HashMap.getElem?_insert]
+          simp [h_rm2_neq_rm, h_rm2_committed]
+        have h: ∃ rm: RM, s'.rmState[rm]? = some RMState.Committed := by
+          exists rm₂
+        simp [h]
 
 /--
  Showing that `invariant` is inductive, that is, it is preserved by the transition relation.
@@ -244,18 +757,52 @@ theorem invariant_is_inductive (s: ProtocolState RM) (s': ProtocolState RM)
       unfold invariant
       apply And.intro
       . exact invariant_is_inductive_tm_abort_lemma1 s s' h_inv h_tm_abort
-      . sorry
-      /-
       . apply And.intro
-        . exact invariant_is_inductive_tm_abort_lemma2 s s' h_inv h_tm_abort
+        . exact invariant_is_inductive_tm_abort_lemma2 s s' h_tm_abort
         . apply And.intro
           . exact invariant_is_inductive_tm_abort_lemma3 s s' h_tm_abort
           . apply And.intro
             . exact invariant_is_inductive_tm_abort_lemma4 s s' h_inv h_tm_abort
             . apply And.intro
-              . exact invariant_is_inductive_tm_abort_lemma5 s s' h_all h_inv h_tm_abort
-              . exact invariant_is_inductive_tm_abort_lemma6 s s' h_tm_abort
-      -/
+              . exact invariant_is_inductive_tm_abort_lemma5 s s' h_tm_abort
+              . exact invariant_is_inductive_tm_abort_lemma6 s s' h_inv h_tm_abort
 
     case inr h_rest =>
-      sorry
+      rcases h_rest with ⟨rm, h_action⟩ -- ∃ rm: RM, action
+      cases h_action
+      case inl h_tm_rcv_prepared =>
+        -- action tm_rcv_prepared
+        apply And.intro
+        . exact invariant_is_inductive_tm_receive_prepared_lemma1 s s' rm h_inv h_tm_rcv_prepared
+        . apply And.intro
+          . exact invariant_is_inductive_tm_receive_prepared_lemma2 s s' rm h_tm_rcv_prepared
+          . apply And.intro
+            . exact invariant_is_inductive_tm_receive_prepared_lemma3 s s' rm h_tm_rcv_prepared
+            . apply And.intro
+              . exact invariant_is_inductive_tm_receive_prepared_lemma4 s s' rm h_inv h_tm_rcv_prepared
+              . apply And.intro
+                . exact invariant_is_inductive_tm_receive_prepared_lemma5 s s' rm h_inv h_tm_rcv_prepared
+                . exact invariant_is_inductive_tm_receive_prepared_lemma6 s s' rm h_all h_inv h_tm_rcv_prepared
+
+      case inr h_rest =>
+        cases h_rest
+        case inl h_rm_prepare =>
+          -- action rm_prepare
+          apply And.intro
+          . exact invariant_is_inductive_rm_prepare_lemma1 s s' rm h_inv h_rm_prepare
+          . apply And.intro
+            . exact invariant_is_inductive_rm_prepare_lemma2 s s' rm h_inv h_rm_prepare
+            . apply And.intro
+              . exact invariant_is_inductive_rm_prepare_lemma3 s s' rm h_inv h_rm_prepare
+              . apply And.intro
+                . exact invariant_is_inductive_rm_prepare_lemma4 s s' rm h_inv h_rm_prepare
+                . apply And.intro
+                  . exact invariant_is_inductive_rm_prepare_lemma5 s s' rm h_inv h_rm_prepare
+                  . exact invariant_is_inductive_rm_prepare_lemma6 s s' rm h_inv h_rm_prepare
+        case inr h_rest =>
+          cases h_rest
+          case inl h_rm_abort =>
+            sorry
+
+          case inr h_rest =>
+            sorry
